src/cbor/pulse/raw/CBOR.Pulse.Raw.Format.Serialize.fsti
@@ -7,15 +7,15 @@ open Pulse.Lib.Trade
 module U8 = FStar.UInt8
 module SZ = FStar.SizeT
 module Trade = Pulse.Lib.Trade.Util
-module S = Pulse.Lib.Slice
+module MS = Pulse.Lib.MutableSlice
 
 val cbor_serialize
   (x: cbor_raw)
-  (output: S.slice U8.t)
+  (output: MS.slice U8.t)
   (#y: Ghost.erased raw_data_item)
   (#pm: perm)
 : stt SZ.t
-    (exists* v . cbor_match pm x y ** pts_to output v ** pure (Seq.length (serialize_cbor y) <= SZ.v (S.len output)))
+    (exists* v . cbor_match pm x y ** pts_to output v ** pure (Seq.length (serialize_cbor y) <= SZ.v (MS.len output)))
     (fun res -> exists* v . cbor_match pm x y ** pts_to output v ** pure (
       let s = serialize_cbor y in
       SZ.v res == Seq.length s /\
